Grw.lean
@@ -4,3 +4,4 @@ import Grw.Morphism
 import Grw.Tactic
 import Grw.PaperTactic
 import Grw.Eauto
+import Grw.Attribute
