Grw/Attribute.lean
@@ -1,0 +1,44 @@
+import Lean
+
+open Lean
+open Lean.Meta
+
+namespace Attribute
+
+initialize
+  Lean.registerTraceClass `Meta.Tactic.grewrite.hints
+
+structure Hint where
+  name : Name
+  keys : Array DiscrTree.Key
+  deriving Inhabited
+
+initialize dbEx : ScopedEnvExtension Hint Hint (DiscrTree Name) ←
+  registerScopedEnvExtension {
+    mkInitial := return {},
+    ofOLeanEntry := fun dt n => do
+      pure n
+    toOLeanEntry := id
+    addEntry := fun dt n => dt.insertCore n.keys n.name,
+    finalizeImport := id,
+  }
+
+private def convertTheoremToHint (name : Name) : MetaM Hint := do
+  let expr ← mkConstWithFreshMVarLevels name
+  let type ← inferType expr
+  let (_, _, type) ← forallMetaTelescope type
+  trace[Meta.Tactic.grewrite.hints]m!"insert: {type}, {name}"
+  let arr ← DiscrTree.mkPath type
+  pure ⟨name, arr⟩
+
+-- For relations create new Attribute (e.g. grewrite_rel) but reuse dbEx
+
+initialize registerBuiltinAttribute {
+  name := `grewrite
+  descr := "Register theorems to be used in the proof search for the grewrite tactic"
+  add := fun name _ kind => do
+    let (hint, _) ← convertTheoremToHint name |>.run
+    dbEx.add hint kind
+}
+
+end Attribute
